Some more cleanup.

Substitution.v
@@ -1,3 +1,14 @@
+(************************************************************************)
+(* Copyright (c) 2010, Martijn Vermaat <martijn@vermaat.name>           *)
+(*                                                                      *)
+(* Licensed under the MIT license, see the LICENSE file or              *)
+(* http://en.wikipedia.org/wiki/Mit_license                             *)
+(************************************************************************)
+
+
+(** This library defines substition of terms for variables in terms. *)
+
+
 Require Export List.
 Require Export FiniteTerm.
 Require Export Term.
@@ -15,36 +26,84 @@ Variable X : variables.
 Notation term := (term F X).
 Notation fterm := (finite_term F X).
 
-(* Type of substitutions of terms for variables *)
+(** A substitution is a function from variables to terms. *)
 Definition substitution := X -> term.
 
-(* Equality of substitutions on a list of variables *)
+(** Equality of substitutions on a list of variables. *)
 Fixpoint substitution_eq (vars : list X) (sigma sigma' : substitution) :=
   match vars with
   | nil     => True
   | x :: xs => (substitution_eq xs sigma sigma') /\ (sigma x = sigma' x)
   end.
 
-(* This equality is reflexive *)
+(** We show this equality is an equivalence. *)
+
 Lemma substitution_eq_refl :
   forall vars sigma, substitution_eq vars sigma sigma.
 Proof.
 induction vars; [simpl | split]; trivial.
 Qed.
 
-(* The identity substitution *)
+Lemma substitution_eq_symm :
+  forall vars sigma theta,
+    substitution_eq vars sigma theta ->
+    substitution_eq vars theta sigma.
+Proof.
+intros vars sigma theta H.
+induction vars as [| x vars IH]; simpl.
+exact I.
+split.
+apply IH.
+apply H.
+symmetry.
+apply H.
+Qed.
+
+Lemma substitution_eq_trans :
+  forall vars sigma theta upsilon,
+    substitution_eq vars sigma theta ->
+    substitution_eq vars theta upsilon ->
+    substitution_eq vars sigma upsilon.
+Proof.
+intros vars sigma theta upsilon H1 H2.
+induction vars as [| x vars IH]; simpl.
+exact I.
+split.
+apply IH.
+apply H1.
+apply H2.
+apply eq_trans with (theta x).
+apply H1.
+apply H2.
+Qed.
+
+(** The identity substitution. *)
 Definition empty_substitution (x : X) : term := Var x.
 
-(* Apply a substitution to a finite term *)
+(** We define two substitution functions. The first, [substitute], defines
+   substitution on finite terms. The second, [substitute'], defines
+   substitution on infinite terms.
+
+   In principle, [substitute'] works fine and is a generalisation of
+   [substitute]. However, it yields a (potentially) infinite term (of type
+   [term] instead of [finite_term]) and this makes it somewhat painful to
+   work with (corecursive definitions have to be manually unfolded in Coq).
+
+   Since we almost always apply substitutions on finite terms, we define
+   this seperately and provide the more general [substitute'] for
+   completeness. *)
+
+(** Apply a substitution to a finite term. *)
 Fixpoint substitute (sigma : substitution) (t : fterm) {struct t} : term :=
   match t with
   | FVar x      => sigma x
   | FFun f args => Fun f (vmap (substitute sigma) args)
   end.
 
-(* Applying the empty substitution to a finite term gives the trivial infinite term image *)
-(* The only reason we cannot prove coq-equality here is equality on vectors *)
-Lemma empty_substitution_is_trivial :
+(** Applying the empty substitution to a finite term gives the trivial
+   infinite term image. The only reason we cannot prove coq-equality here
+   is equality on vectors. *)
+Lemma empty_substitution_is_id :
   forall (t : fterm), substitute empty_substitution t [~] t.
 Proof.
 induction t.
@@ -53,28 +112,19 @@ constructor.
 assumption.
 Qed.
 
-(* TODO: with the recursive vectors we can also define this as a cofixpoint on
-   (non-finite) terms. Below are some additional lemmas for reassurance. *)
+(** Apply a substitution to an infinite term. Note that this definition is
+   not in guarded form if we were to use the inductive vector type from the
+   standard library. It is in guarded form here, because we use [vector]
+   from the [Vector] library, where [vmap] is just an abstraction (which
+   ensures the corecursive call to [substitute'] to be guarded). *)
 CoFixpoint substitute' (sigma : substitution) (t : term) : term :=
   match t with
   | Var x      => sigma x
   | Fun f args => Fun f (vmap (substitute' sigma) args)
   end.
 
-(* Take apart a coinductive term up to depth 1 and put it back together *)
-(* TODO: move to Term.v *)
-Definition peek (t : term) : term :=
-  match t with
-  | Var x      => Var x
-  | Fun f args => Fun f args
-  end.
-
-Lemma peek_eq : forall (t : term), t = peek t.
-  destruct t; reflexivity.
-Qed.
-
-(* Applying the empty substitution to a finite term gives the trivial infinite term image *)
-Lemma empty_substitution_is_trivial' :
+(** Applying the empty substitution to a term gives the same term. *)
+Lemma empty_substitution_is_id' :
   forall (t : term), substitute' empty_substitution t [~] t.
 Proof.
 cofix IH.
@@ -89,8 +139,9 @@ unfold vmap.
 apply IH.
 Qed.
 
-(* the following can be proved for coq-equality were it not that
-   we cannot equate (vmap finite_term_as_term v) and v *)
+(** We prove that both substitution functions do the same thing (on finite
+   terms). We can almost prove this for coq-equality, but we cannot equate
+   [vmap finite_term_as_term v] and [v]. *)
 Lemma substitutions_related :
   forall (s : substitution) (t : fterm), substitute s t [~] substitute' s t.
 Proof.
